\documentclass{article}
\usepackage[utf8]{inputenc}
\usepackage{amsmath}

\title{QUBO to Ising Hamiltonian Model Transformation}
\author{}
\date{\today}

\begin{document}

\maketitle
Starting from the equation (13) from the paper, we have the following QUBO problem:
\begin{equation}
	\max_{b} L(b) = \max_{b} \left(\mu''^Tb -qb^T\Sigma''b \underbrace{- \lambda(P''^T b-1)^2}_{penalty}\right)
\end{equation}
Now we expand its component:
\begin{align}
	\mu''^Tb              & = \sum_{i}^{} u''_i b_i,                             \\
	-qb^T\Sigma''b        & = -q \sum_{i,j}^{} \Sigma''_{ij} b_i b_j,            \\
	-\lambda(P''^T b-1)^2 & = -\lambda \left(\sum_{i}^{} P''_i b_i - 1\right)^2.
\end{align}
We have the transformation of \(b_i = \frac{1+s_i}{2}; b_j = \frac{1+s_j}{2}\)
\begin{align}
	\sum_{i}^{} u''_i b_i & = \sum_{i}^{} u''_i \frac{1+s_i}{2}                                  \\
	                      & = \underbrace{\frac{1}{2} \sum_{i}^{} u''_i} + \underbrace{\frac{1}{2} \sum_{i}^{} u''_i s_i}, 
\end{align}
Substitute \(b_ib_j\)
\begin{equation}
	b_ib_j = \frac{1+s_i}{2} \cdot \frac{1+s_j}{2}  = \frac{(1+s_i)(1+s_j)}{4} = \frac{1}{4}(1 + s_i + s_j + s_is_j)
\end{equation}
\begin{align}
	-q \sum_{i,j}^{} \Sigma''_{ij} b_i b_j & = -q \sum_{i,j}^{} \Sigma''_{ij} \frac{1}{4}(1 + s_i + s_j + s_is_j)                                                                                                                   \\
	                                       & = \underbrace{-\frac{q}{4} \sum_{i,j}^{} \Sigma''_{ij}} \underbrace{-\frac{q}{4} \sum_{i,j}^{} \Sigma''_{ij} s_i - \frac{q}{4} \sum_{i,j}^{} \Sigma''_{ij} s_j} \underbrace{- \frac{q}{4} \sum_{i,j}^{} \Sigma''_{ij} s_is_j}
\end{align}
Since \(\Sigma''\) is symmetric, we have:
\begin{equation}
	-\frac{q}{4} \sum_{i,j}^{} \Sigma''_{ij} s_i -\frac{q}{4} \sum_{i,j}^{} \Sigma''_{ij} s_j = -\frac{q}{2} \sum_{i}^{} \left(\sum_{j}^{}\Sigma''_{ij}\right) s_i
\end{equation}
Penalty term:
\begin{align}
    -\lambda \left(\sum_{i}^{} P''_i b_i - 1\right)^2 &= -\lambda \left(\sum_{i}^{} P''_i \frac{1+s_i}{2} - 1\right)^2 \\
    &= -\lambda \left(\frac{1}{2} \sum_{i}^{}P''_i(1+s_i) -1\right)^2 \\
    &= -\lambda \left(\frac{1}{2} \sum_{i}^{}P''_i + \frac{1}{2} \sum_{i}^{}P''_i s_i - 1\right)^2 
\end{align}
According to equation (15) from the paper, we have the penalty term in the as:
\begin{equation}
    +\lambda \left(\sum_{i}^{}\pi_i s_i - \beta\right)^2 
\end{equation}
Let $\pi_i = \frac{1}{2} P''_i\) and \(\beta = 1-\frac{1}{2} \sum_{i}^{} P''_i $, equation (13) can be written as (flip the sign to convert maximization to minimization):
\begin{align}
    &+\lambda \left(\sum_{i}^{}\pi_i s_i - \beta\right)^2 \\
    &= \lambda \left(\left(\sum_{i}^{}\pi_i s_i\right)^2 - 2 \left(\sum_{i}^{}\pi_i s_i\right)\beta + \beta^2 \right) \\
\end{align}
The Ising objective function from the paper is written as:
\begin{equation}
    \min_{s} L(s) : \min_s \left(\sum_{i}^{}h_i s_i + \sum_{i,j}^{}J_{i,j} s_i s_j + \lambda \left(\sum_{i}^{}\pi_i s_i - \beta\right)^2\right),
\end{equation}
\begin{equation*}
    \text{s.t} \quad s_{i,j} \in \{-1, 1\} \quad \forall i,j
\end{equation*}
From equations (6), (9) , (10), we can derive $h$ , $J$, and other constant as:
\begin{align}
    h_i & = \frac{1}{2} \mu''_i -\frac{q}{2} \sum_{j}^{}\Sigma''_{ij}\\
    J_{i,j} & = -\frac{q}{4} \Sigma''_{i,j} \\
    \text{Constant} &= \frac{1}{2} \sum_{i}^{} u''_i - \frac{q}{4} \sum_{i,j}^{} \Sigma''_{ij} 
\end{align}
\end{document}